Define closing, prove OC1-OC9 from the paper and find nice notations for opening and closing.

LocallyNameless/STLC.v
@@ -15,7 +15,7 @@ Parameters
 Existing Instance Decidable_eq_Atom.
 
 Inductive Tm : Type :=
-| fvar : Atom -> Tm
+| fvar (a : Atom) : Tm
 | bvar : nat -> Tm
 | abs  : Tm -> Tm
 | app  : Tm -> Tm -> Tm.
@@ -47,7 +47,7 @@ Notation "x |> f" := (f x) (at level 68, only parsing).
 
 (* Notation "t [ x ~> u ]" := (subst x u t) (at level 68). *)
 
-Notation "t [ x := u ]" := (subst x u t) (at level 68).
+Notation "t [[ x := u ]]" := (subst x u t) (at level 68).
 
 Lemma subst_demo :
   forall x y : Atom,
@@ -90,44 +90,44 @@ Proof.
     now destruct IHt1, IHt2; firstorder congruence.
 Qed.
 
-Fixpoint open_aux (i : nat) (u t : Tm) : Tm :=
+Fixpoint open (i : nat) (u t : Tm) : Tm :=
 match t with
 | fvar a    => fvar a
 | bvar j    => if decide (i = j) then u else bvar j
-| abs t'    => abs (open_aux (S i) u t')
-| app t1 t2 => app (open_aux i u t1) (open_aux i u t2)
+| abs t'    => abs (open (S i) u t')
+| app t1 t2 => app (open i u t1) (open i u t2)
 end.
 
-(* Notation "{ n ~> t2 } t1" := (open_aux t1 n t2) (at level 68). *)
-Notation "t { i ~> u }" := (open_aux i u t) (at level 68).
+(* Notation "{ n ~> t2 } t1" := (open t1 n t2) (at level 68). *)
+Notation "t {{ i ~> u }}" := (open i u t) (at level 68).
 
-Definition open (u t : Tm) : Tm :=
-  open_aux 0 u t.
+Definition open' (u t : Tm) : Tm :=
+  open 0 u t.
 
 Lemma open_demo :
   forall y : Atom,
-    app (abs (app 1 0)) 0 |> open y = app (abs (app y 0)) y.
+    app (abs (app 1 0)) 0 |> open' y = app (abs (app y 0)) y.
 Proof.
   easy.
 Qed.
 
 Inductive lc : Tm -> Prop :=
 | lc_fvar : forall x : Atom, lc x
-| lc_abs  : forall (t : Tm) (x : Atom), lc (open x t)  -> lc (abs t)
+| lc_abs  : forall (t : Tm) (x : Atom), lc (open' x t)  -> lc (abs t)
 | lc_app  : forall t1 t2 : Tm, lc t1 -> lc t2 -> lc (app t1 t2).
 
 #[export] Hint Constructors lc : core.
 
-Lemma open_aux_open_aux :
-  forall (t : Tm) (n m : nat) (u1 u2 : Tm),
-    n <> m ->
-    t |> open_aux n u1 |> open_aux m u2 = t |> open_aux n u1 ->
-      t |> open_aux m u2 = t.
+Lemma open_open :
+  forall (t : Tm) (i j : nat) (u1 u2 : Tm),
+    i <> j ->
+    t {{ i ~> u1 }} {{ j ~> u2 }} = t {{ i ~> u1 }} ->
+      t {{ j ~> u2 }} = t.
 Proof.
   induction t; cbn; intros * Hneq H.
   - easy.
-  - destruct (PeanoNat.Nat.eqb_spec n0 n); [| easy].
-    destruct (PeanoNat.Nat.eqb_spec m n); [| easy].
+  - destruct (PeanoNat.Nat.eqb_spec i n); [| easy].
+    destruct (PeanoNat.Nat.eqb_spec j n); [| easy].
     now congruence.
   - inversion H.
     f_equal.
@@ -139,56 +139,56 @@ Proof.
     + now eapply IHt2, H2.
 Qed.
 
-Lemma open_aux_open :
-  forall (t : Tm) (n : nat) (x : Atom) (u : Tm),
-    t |> open x |> open_aux (S n) u = t |> open x ->
-      t |> open_aux (S n) u = t.
+Lemma open_open' :
+  forall (t : Tm) (i : nat) (x : Atom) (u : Tm),
+(*     t |> open' x |> open (S i) u = t |> open' x -> *)
+    t {{ 0 ~> x }} {{ S i ~> u }} = t {{ 0 ~> x }} ->
+      t {{ S i ~> u }} = t.
 Proof.
-  unfold open.
+  unfold open'.
   intros.
-  now apply open_aux_open_aux in H.
+  now apply open_open in H.
 Qed.
 
-Lemma open_aux_lc :
-  forall (t : Tm) (n : nat) (u : Tm),
-    lc t -> t |> open_aux n u = t.
+Lemma open_lc :
+  forall (t : Tm) (i : nat) (u : Tm),
+    lc t -> t {{ i ~> u }} = t.
 Proof.
   intros t n u Hlc; revert n u.
   induction Hlc; cbn; intros; [easy | |].
   - f_equal.
-    now eapply open_aux_open, IHHlc.
+    now eapply open_open', IHHlc.
   - now f_equal.
 Qed.
 
-Lemma subst_open_aux :
-  forall (t : Tm) (n : nat) (u1 : Tm) (x : Atom) (u2 : Tm),
+Lemma subst_open :
+  forall (t : Tm) (i : nat) (u1 : Tm) (x : Atom) (u2 : Tm),
     lc u2 ->
-    t |> open_aux n u1 |> subst x u2
+    t {{ i ~> u1 }} [[ x := u2 ]]
       =
-    t |> subst x u2 |> open_aux n (u1 |> subst x u2).
+    t [[ x := u2 ]] {{ i ~> u1 [[ x := u2 ]] }}.
 Proof.
   induction t; cbn; intros.
-  - rewrite open_aux_lc; [easy |].
+  - rewrite open_lc; [easy |].
     now decide (x = a).
-  - now destruct (PeanoNat.Nat.eqb n0 n).
+  - now destruct (PeanoNat.Nat.eqb i n).
   - now rewrite IHt.
   - now rewrite IHt1, IHt2.
 Qed.
 
 Lemma open_subst :
-  forall (t : Tm) (x y : Atom) (u : Tm),
-    x <> y -> lc u ->
-      t |> subst x u |> open y = t |> open y |> subst x u.
+  forall (t : Tm) (a b : Atom) (u : Tm),
+    a <> b -> lc u ->
+    t [[ a := u ]] {{ 0 ~> b }} = t {{ 0 ~> b }} [[ a := u ]].
 Proof.
-  unfold open.
   intros.
-  rewrite subst_open_aux; cbn; [| easy].
-  now decide (x = y).
+  rewrite subst_open; cbn; [| easy].
+  now decide (a = b).
 Qed.
 
 Lemma lc_subst :
-  forall (t : Tm) (x : Atom) (u : Tm),
-    lc t -> lc u -> lc (subst x u t).
+  forall (t : Tm) (a : Atom) (u : Tm),
+    lc t -> lc u -> lc (t [[ a := u ]]).
 Proof.
   intros t x u Ht Hu; revert x u Hu.
   induction Ht; cbn; intros.
@@ -196,3 +196,173 @@ Proof.
   - admit.
   - now constructor; firstorder.
 Abort.
+
+Fixpoint succ (t : Tm) : Tm :=
+match t with
+| fvar x    => fvar x
+| bvar i    => bvar (S i)
+| abs t'    => abs t'
+| app t1 t2 => app (succ t1) (succ t2)
+end.
+
+(*
+Fixpoint close (a : Atom) (u t : Tm) : Tm :=
+match t with
+| fvar x    => if decide (a = x) then u else fvar x
+| bvar i    => bvar i
+| abs t'    => abs (close a (succ u) t')
+| app t1 t2 => app (close a u t1) (close a u t2)
+end.
+
+Notation "t {{ u <~ a }}" := (close a u t) (at level 68).
+*)
+
+Fixpoint close (a : Atom) (i : nat) (t : Tm) : Tm :=
+match t with
+| fvar x    => if decide (a = x) then bvar i else fvar x
+| bvar n    => bvar n
+| abs t'    => abs (close a (S i) t')
+| app t1 t2 => app (close a i t1) (close a i t2)
+end.
+
+Notation "t {{ i <~ a }}" := (close a i t) (at level 68).
+
+(* OC 1 *)
+Lemma open_open_eq :
+  forall (t : Tm) (i : nat) (a b : Atom),
+    t {{ i ~> a }} {{ i ~> b }} = t {{ i ~> a }}.
+Proof.
+  induction t; cbn; intros; [easy | | |].
+  - destruct (PeanoNat.Nat.eqb_spec i n); cbn; [easy |].
+    now destruct (PeanoNat.Nat.eqb_spec i n).
+  - now rewrite IHt.
+  - now rewrite IHt1, IHt2.
+Qed.
+
+(* OC 2 *)
+Lemma close_close_eq :
+  forall (t : Tm) (a : Atom) (i j : nat),
+    t {{ i <~ a }} {{ j <~ a }} = t {{ i <~ a }}.
+Proof.
+  induction t; cbn; intros; [| easy | |].
+  - decide (a0 = a); cbn; [easy |].
+    now decide (a0 = a).
+  - now rewrite IHt.
+  - now rewrite IHt1, IHt2.
+Qed.
+
+(* OC 3 *)
+Lemma open_close_eq :
+  forall (t : Tm) (i : nat) (a : Atom),
+    t {{ i ~> a }} {{ i <~ a }} = t {{ i <~ a }}.
+Proof.
+  induction t; cbn; intros; [easy | ..].
+  - destruct (PeanoNat.Nat.eqb_spec i n); subst; cbn; [| easy].
+    now decide (a = a).
+  - now rewrite IHt.
+  - now rewrite IHt1, IHt2.
+Qed.
+
+(* OC 4 *)
+Lemma close_open_eq :
+  forall (t : Tm) (i : nat) (a : Atom),
+    t {{ i <~ a }} {{ i ~> a }} = t {{ i ~> a }}.
+Proof.
+  induction t; cbn; intros; [| easy | ..].
+  - decide (a0 = a); subst; cbn; [| easy].
+    now destruct (PeanoNat.Nat.eqb_spec i i).
+  - now rewrite IHt.
+  - now rewrite IHt1, IHt2.
+Qed.
+
+(* OC 5 *)
+Lemma open_open_neq :
+  forall (t : Tm) (i j : nat) (a b : Atom),
+    i <> j ->
+      t {{ i ~> a }} {{ j ~> b }} = t {{ j ~> b }} {{ i ~> a }}.
+Proof.
+  induction t; cbn; intros; [easy | ..].
+  - destruct (PeanoNat.Nat.eqb_spec j n); cbn;
+      destruct (PeanoNat.Nat.eqb_spec i n); subst; cbn; [easy | | easy |].
+    + now destruct (PeanoNat.Nat.eqb_spec n n).
+    + now destruct (PeanoNat.Nat.eqb_spec j n).
+  - now rewrite IHt; [| congruence].
+  - now rewrite IHt1, IHt2.
+Qed.
+
+(* OC 6 *)
+Lemma close_close_neq :
+  forall (t : Tm) (i j : nat) (a b : Atom),
+    a <> b ->
+      t {{ i <~ a }} {{ j <~ b }} = t {{ j <~ b }} {{ i <~ a }}.
+Proof.
+  induction t; cbn; intros; [| easy | ..].
+  - decide (a0 = a); subst; cbn;
+      decide (b = a); subst; cbn; only 1, 3: easy.
+    + now decide (a = a).
+    + now decide (a0 = a).
+  - now rewrite IHt; [| congruence].
+  - now rewrite IHt1, IHt2.
+Qed.
+
+(* OC 7 *)
+Lemma open_close_neq :
+  forall (t : Tm) (i j : nat) (a b : Atom),
+    i <> j -> a <> b ->
+      t {{ i ~> a }} {{ j <~ b }} = t {{ j <~ b }} {{ i ~> a }}.
+Proof.
+  induction t; cbn; intros.
+  - decide (b = a); subst; cbn; [| easy].
+    now destruct (PeanoNat.Nat.eqb_spec i j).
+  - destruct (PeanoNat.Nat.eqb_spec i n); cbn; [| easy].
+    now decide (b = a); subst.
+  - now rewrite IHt; congruence.
+  - now rewrite IHt1, IHt2.
+Qed.
+
+(* OC 8 *)
+Lemma open_close_open :
+  forall (t : Tm) (i j : nat) (a b : Atom),
+    t {{ i ~> a }} {{ j <~ a }} {{ j ~> b }}
+      =
+    t {{ j ~> b }} {{ i <~ a }} {{ i ~> b }}.
+Proof.
+  induction t; cbn; intros.
+  - decide (a0 = a); cbn; [| easy].
+    now destruct (PeanoNat.Nat.eqb_spec j j), (PeanoNat.Nat.eqb_spec i i).
+  - destruct (PeanoNat.Nat.eqb_spec i n); subst; cbn;
+      destruct (PeanoNat.Nat.eqb_spec j n); subst; cbn.
+    + rewrite Decidable_complete by easy.
+      now decide (a = b); cbn; destruct (PeanoNat.Nat.eqb_spec n n).
+    + rewrite Decidable_complete by easy; cbn.
+      now destruct (PeanoNat.Nat.eqb_spec j j), (PeanoNat.Nat.eqb_spec n n).
+    + decide (a = b); cbn; [| easy].
+      now destruct (PeanoNat.Nat.eqb_spec i i).
+    + now destruct (PeanoNat.Nat.eqb_spec i n).
+  - now rewrite IHt.
+  - now rewrite IHt1, IHt2.
+Qed.
+
+(* OC 9 *)
+Lemma close_open_close :
+  forall (t : Tm) (i j : nat) (a b : Atom),
+    t {{ i <~ a }} {{ i ~> b }} {{ j <~ b }}
+      =
+    t {{ j <~ b }} {{ i ~> a }} {{ j <~ a }}.
+Proof.
+  induction t; cbn; intros.
+  - decide (b = a); subst; cbn; decide (a0 = a); subst; cbn.
+    + now destruct (PeanoNat.Nat.eqb_spec i j), (PeanoNat.Nat.eqb_spec i i); cbn;
+        rewrite ?Decidable_complete by easy.
+    + rewrite Decidable_complete by easy.
+      destruct (PeanoNat.Nat.eqb_spec i j); cbn; [| easy].
+      now rewrite Decidable_complete.
+    + destruct (PeanoNat.Nat.eqb_spec i i); cbn; [| easy].
+      now rewrite Decidable_complete.
+    + now decide (b = a).
+  - destruct (PeanoNat.Nat.eqb_spec i n); subst; cbn; [| easy].
+    now rewrite !Decidable_complete.
+  - now rewrite IHt.
+  - now rewrite IHt1, IHt2.
+Qed.
+
